FGL: global transforms certify

books/centaur/fgl/aignet-pathcond-stobj.lisp
@@ -33,14 +33,144 @@
 (include-book "centaur/aignet/mark-impls" :dir :system)
 (include-book "centaur/misc/intstack" :dir :system)
 (include-book "centaur/fty/baselists" :dir :system)
+(include-book "centaur/misc/starlogic" :dir :system)
 (local (include-book "theory"))
 (local (std::add-default-post-define-hook :fix))
 
 
 
-(fty::defalist nbalist :pred nbalistp :key-type posp :val-type bitp :true-listp t :unique-keys t)
+;; (fty::defalist nbalist :pred nbalistp :key-type natp :val-type bitp :true-listp t :unique-keys t)
+(define nbalistp (x)
+  (if (atom x)
+      (eq x nil)
+    (and (consp (car x))
+         (not (hons-assoc-equal (caar x) (cdr x)))
+         (natp (caar x))
+         (bitp (cdar x))
+         (not (equal (car x) '(0 . 0)))
+         (nbalistp (cdr x))))
+  ///
+  (defthm nbalistp-of-cdr
+    (implies (nbalistp x)
+             (nbalistp (cdr x)))
+    :hints (("goal" :expand ((nbalistp x)))))
+  (defthm natp-of-caar-when-nbalistp
+    (implies (and (nbalistp x) (consp x))
+             (natp (caar x)))
+    :hints (("goal" :expand ((nbalistp x)))))
+  (defthm bitp-of-cdar-when-nbalistp
+    (implies (and (nbalistp x) (consp x))
+             (bitp (cdar x)))
+    :hints (("goal" :expand ((nbalistp x)))))
+  (defthm
+    nbalistp-of-cons
+    (equal (nbalistp (cons a x))
+           (and (and (consp a)
+                     (natp (car a))
+                     (bitp (cdr a))
+                     (not (hons-assoc-equal (car a) x))
+                     (not (equal a '(0 . 0))))
+                (nbalistp x)))
+    :hints (("goal" :expand ((nbalistp (cons a x)))))))
 
-(fty::deflist pos-list :elt-type posp :true-listp t)
+(define nbalist-fix ((x nbalistp))
+  :returns (new-x nbalistp
+                  :hints ('(:in-theory (disable nbalist-fix nbalistp)
+                            :expand ((nbalist-fix x)
+                                     (:free (a b) (nbalistp (cons a b)))
+                                     (nbalistp x)
+                                     (nbalistp nil)))))
+  :inline t
+  :verify-guards nil
+  (mbe :logic (if (atom x)
+                  nil
+                (let
+                    ((rest (nbalist-fix (cdr x))))
+                  (if (and (consp (car x)))
+                      (let ((first-key (nfix (caar x)))
+                            (first-val (bfix (cdar x))))
+                        (if (or (hons-assoc-equal first-key rest)
+                                (and (equal first-key 0)
+                                     (equal first-val 0)))
+                            rest
+                          (cons (cons first-key first-val)
+                                rest)))
+                    rest)))
+       :exec x)
+  ///
+  (local (in-theory (disable (:d nbalist-fix))))
+  (defthm
+    nbalist-fix-when-nbalistp
+    (implies (nbalistp x)
+             (equal (nbalist-fix x) x))
+    :hints
+    ('(:expand ((nbalistp x) (nbalist-fix x))
+       :in-theory (disable nbalist-fix nbalistp))))
+  (verify-guards+ nbalist-fix
+                  :hints (("goal" :expand ((nbalistp x)))))
+  (defsection
+    nbalist-equiv :parents (nbalist)
+    (fty::deffixtype nbalist
+      :pred nbalistp
+      :fix nbalist-fix
+      :equiv nbalist-equiv
+      :define t
+      :forward t))
+  (local (in-theory (enable nbalist-equiv)))
+  (fty::deffixcong
+    acl2::nat-equiv
+    nbalist-equiv (cons (cons k v) x)
+    k
+    :pkg nbalist-equiv
+    :hints
+    (("goal" :expand ((:free (a b)
+                       (nbalist-fix (cons a b)))))))
+  (fty::deffixcong
+    acl2::bit-equiv
+    nbalist-equiv (cons (cons k v) x)
+    v
+    :pkg nbalist-equiv
+    :hints
+    (("goal" :expand ((:free (a b)
+                       (nbalist-fix (cons a b)))))))
+  (fty::deffixcong
+    nbalist-equiv nbalist-equiv (cons x y)
+    y
+    :pkg nbalist-equiv
+    :hints
+    (("goal" :expand ((:free (a b)
+                       (nbalist-fix (cons a b)))))))
+  (defthm
+    nbalist-fix-of-acons
+    (equal
+     (nbalist-fix (cons (cons a b) x))
+     (let
+         ((rest (nbalist-fix x)))
+       (if
+           (and)
+           (let ((first-key (nfix a))
+                 (first-val (bfix b)))
+             (if (or (hons-assoc-equal first-key rest)
+                     (and (equal first-key 0) (equal first-val 0)))
+                 rest
+               (cons (cons first-key first-val)
+                     rest)))
+         rest)))
+    :hints
+    (("goal" :expand ((:free (a b)
+                       (nbalist-fix (cons a b)))))))
+  (defthm
+    consp-car-of-nbalist-fix
+    (equal (consp (car (nbalist-fix x)))
+           (consp (nbalist-fix x)))
+    :hints
+    (("goal"
+      :induct (len x)
+      :expand ((nbalist-fix x))
+      :in-theory (e/d ((:i len)) ((:d nbalist-fix)))))))
+  
+
+(fty::deflist pos-list :elt-type natp :true-listp t)
 
 
 (local (defthm cdr-hons-assoc-equal-when-nbalistp
@@ -55,28 +185,119 @@
   (nbalist-bits$c :type bitarr)
   (nbalist-stack$c :type acl2::intstack))
 
+
+(local (defthm nat-listp-when-u32-listp
+         (implies (acl2::u32-listp x)
+                  (nat-listp x))))
+
+(define nbalist-stobj-zero-unbound-aux (acl2::intstack bitarr)
+  (implies (mbe :logic (consp (non-exec (member 0 (acl2::nat-list-fix acl2::intstack))))
+                :exec (acl2::intstack-member^ 0 acl2::intstack))
+           (mbe :logic (equal (get-bit 0 bitarr) 1)
+                :exec (and (< 0 (bits-length bitarr))
+                           (equal (get-bit 0 bitarr) 1))))
+  ///
+  (defthm nbalist-stobj-zero-unbound-aux-implies
+    (implies (and (nbalist-stobj-zero-unbound-aux intstack bitarr)
+                  (member 0 (acl2::nat-list-fix intstack)))
+             (equal (nth 0 bitarr) 1))
+    :rule-classes :forward-chaining)
+
+  (defthm nbalist-stobj-zero-unbound-aux-implies-no-fix
+    (implies (and (nbalist-stobj-zero-unbound-aux intstack bitarr)
+                  (member 0 intstack)
+                  (acl2::u32-listp intstack))
+             (equal (nth 0 bitarr) 1))
+    :rule-classes :forward-chaining)
+
+  (defthm nbalist-stobj-zero-unbound-aux-implies-nth
+    (implies (and (equal (nth n (acl2::nat-list-fix intstack)) 0)
+                  (not (equal (nth 0 bitarr) 1)))
+             (not (nbalist-stobj-zero-unbound-aux intstack bitarr)))
+    :hints (("goal" :use ((:instance acl2::member-of-nth
+                           (n n) (x (acl2::nat-list-fix intstack)))))))
+
+  (local (defthm nth-of-nat-listp-when-zp-nth
+           (implies (and (zp (nth n x))
+                         (< (nfix n) (len x)))
+                    (equal (nth n (acl2::nat-list-fix x)) 0))
+           :hints(("Goal" :in-theory (enable acl2::nat-list-fix nth)))))
+
+  (defthm nbalist-stobj-zero-unbound-aux-implies-nth-unfix
+    (implies (and (zp (nth n intstack))
+                  (< (nfix n) (len intstack))
+                  (not (equal (nth 0 bitarr) 1)))
+             (not (nbalist-stobj-zero-unbound-aux intstack bitarr)))
+    :hints (("goal" :use ((:instance acl2::member-of-nth
+                           (n n) (x (acl2::nat-list-fix intstack))))
+             :in-theory (disable acl2::member-of-nth))))
+
+  (defthmd nbalist-stobj-zero-unbound-aux-expand
+    (equal (nbalist-stobj-zero-unbound-aux intstack bitarr)
+           (if (atom intstack)
+               t
+             (and (or (posp (car intstack))
+                      (equal (nth 0 bitarr) 1))
+                  (nbalist-stobj-zero-unbound-aux (cdr intstack) bitarr))))
+    :hints(("Goal" :in-theory (enable acl2::nat-list-fix)))
+    :rule-classes :definition)
+
+  (defthm nbalist-stobj-zero-unbound-aux-of-nat-list-fix
+    (equal (nbalist-stobj-zero-unbound-aux (acl2::nat-list-fix stack) bits)
+           (nbalist-stobj-zero-unbound-aux stack bits)))
+
+  (defthm nbalist-stobj-zero-unbound-aux-of-update-nonzero-bit
+    (implies (not (zp id))
+             (equal (nbalist-stobj-zero-unbound-aux stack (update-nth id val bits))
+                    (nbalist-stobj-zero-unbound-aux stack bits))))
+
+  (defthm nbalist-stobj-zero-unbound-aux-of-resize-bits
+    (implies (< 0 (nfix len))
+             (equal (nbalist-stobj-zero-unbound-aux stack (resize-list bits len 0))
+                    (nbalist-stobj-zero-unbound-aux stack bits))))
+
+  (defthm nbalist-stobj-zero-unbound-aux-of-set-0-1
+    (nbalist-stobj-zero-unbound-aux stack (update-nth 0 1 bits))))
+
+(define nbalist-stobj-zero-unbound (nbalist-stobj$c)
+  :enabled t
+  (stobj-let ((acl2::intstack (nbalist-stack$c nbalist-stobj$c))
+              (bitarr (nbalist-bits$c nbalist-stobj$c)))
+             (ok)
+             (nbalist-stobj-zero-unbound-aux acl2::intstack bitarr)
+             ok))
+
 (define nbalist-stobj-nbalist$c-logic ((stack acl2::intstack$ap)
                                         (bits bit-listp))
   :returns (nbalist)
   (if (atom stack)
       nil
-    (cons (b* ((elt (pos-fix (car stack))))
-            (cons elt (bfix (nth elt bits))))
+    (b* ((elt (nfix (car stack)))
+         (bit (bfix (nth elt bits)))
+         ((when (and (eql elt 0)
+                     (eql bit 0)))
           (nbalist-stobj-nbalist$c-logic (cdr stack) bits)))
+    (cons (cons elt bit)
+          (nbalist-stobj-nbalist$c-logic (cdr stack) bits))))
   ///
   (defret lookup-in-nbalist-stobj-nbalist$c-logic
     (equal (hons-assoc-equal key nbalist)
-           (and (posp key)
-                (member key (pos-list-fix stack))
+           (and (natp key)
+                (member key (acl2::nat-list-fix stack))
+                (implies (equal key 0)
+                         (equal (nth key bits) 1))
                 (cons key (bfix (nth key bits))))))
 
   (defret nbalistp-of-nbalist-stobj-nbalist$c-logic
-    (implies (no-duplicatesp-equal (pos-list-fix stack))
+    (implies (no-duplicatesp-equal (acl2::nat-list-fix stack))
              (nbalistp nbalist)))
   
   (defret len-of-<fn>
-    (equal (len nbalist)
-           (len stack)))
+    (implies (nbalist-stobj-zero-unbound-aux stack bits)
+             (equal (len nbalist)
+                    (len stack)))
+    :hints(("Goal" :induct (len stack)
+            :expand ((nbalist-stobj-zero-unbound-aux stack bits)))))
 
   (local (defthm nth-of-bit-list-fix
            (bit-equiv (nth n (bit-list-fix x))
@@ -84,7 +305,7 @@
            :hints(("Goal" :in-theory (enable nth)))))
 
   (defthm nbalist-stobj-nbalist$c-logic-of-update-non-member
-    (implies (not (member-equal (nfix n) (pos-list-fix stack)))
+    (implies (not (member-equal (nfix n) (acl2::nat-list-fix stack)))
              (equal (nbalist-stobj-nbalist$c-logic stack (update-nth n val bits))
                     (nbalist-stobj-nbalist$c-logic stack bits))))
 
@@ -93,53 +314,30 @@
              (equal (nbalist-stobj-nbalist$c-logic stack (resize-list bits n 0))
                     (nbalist-stobj-nbalist$c-logic stack bits))))
 
-  (defthm nbalist-stobj-nbalist$c-logic-of-pos-list-fix
-    (equal (nbalist-stobj-nbalist$c-logic (pos-list-fix stack) bits)
+  (defthm nbalist-stobj-nbalist$c-logic-of-nat-list-fix
+    (equal (nbalist-stobj-nbalist$c-logic (acl2::nat-list-fix stack) bits)
            (nbalist-stobj-nbalist$c-logic stack bits))
-    :hints(("Goal" :in-theory (enable pos-list-fix))))
+    :hints(("Goal" :in-theory (enable acl2::nat-list-fix))))
 
   (defthm nth-of-nbalist-stobj-nbalist$c-logic
-    (equal (nth n (nbalist-stobj-nbalist$c-logic stack bits))
-           (and (< (nfix n) (len stack))
-                (cons (pos-fix (nth n stack))
-                      (bfix (nth (pos-fix (nth n stack)) bits)))))
-    :hints(("Goal" :in-theory (enable nth)))))
+    (implies (nbalist-stobj-zero-unbound-aux stack bits)
+             (equal (nth n (nbalist-stobj-nbalist$c-logic stack bits))
+                    (and (< (nfix n) (len stack))
+                         (cons (nfix (nth n stack))
+                               (bfix (nth (nfix (nth n stack)) bits))))))
+    :hints(("Goal" :in-theory (enable nth)
+            :induct (nth n stack)
+            :expand ((nbalist-stobj-zero-unbound-aux stack bits))))))
 
 
-(local (defthm nat-listp-when-u32-listp
-         (implies (acl2::u32-listp x)
-                  (nat-listp x))))
 
-
-(local (in-theory (disable acl2::posp-redefinition posp)))
-
-(local (Defthm posp-of-nfix
-         (equal (posp (nfix x))
-                (posp x))
-         :hints(("Goal" :in-theory (enable nfix)))))
-
-(local (Defthm pos-fix-of-nfix
-         (equal (pos-fix (nfix x))
-                (pos-fix x))
-         :hints(("Goal" :in-theory (enable nfix pos-fix)))))
-
-(local (defthm posp-nth-when-u32-listp
-         (implies (and (acl2::u32-listp x)
-                       (not (member 0 x))
-                       (< (nfix n) (len x)))
-                  (posp (nth n x)))
-         :hints(("Goal" :in-theory (enable acl2::u32-listp nth)))))
-
-(local (defthm natp-when-posp
-         (implies (posp x)
-                  (natp x))))
 
 (define nbalist-stobj-nbalist$c-aux ((n natp)
                                       acl2::intstack
                                       bitarr)
   :measure (nfix (- (acl2::intstack-count acl2::intstack) (nfix n)))
   :guard (and (<= n (acl2::intstack-count acl2::intstack))
-              (not (acl2::intstack-member 0 acl2::intstack)))
+              (nbalist-stobj-zero-unbound-aux acl2::intstack bitarr))
   :returns (nbalist (equal nbalist
                            (nbalist-stobj-nbalist$c-logic (nthcdr n acl2::intstack) bitarr))
                     :hints(("Goal" :induct t)
@@ -163,31 +361,19 @@
   (if (mbe :logic (zp (nfix (- (acl2::intstack-count acl2::intstack) (nfix n))))
            :exec (eql n (acl2::intstack-count acl2::intstack)))
       nil
-    (b* ((elt (lposfix (acl2::intstack-nth n acl2::intstack)))
+    (b* ((elt (lnfix (acl2::intstack-nth n acl2::intstack)))
          (bit (mbe :logic (get-bit elt bitarr)
                    :exec (if (< elt (bits-length bitarr))
                              (get-bit elt bitarr)
-                           0))))
+                           0)))
+         ((unless (mbt (not (and (eql elt 0) (eql bit 0)))))
+          (nbalist-stobj-nbalist$c-aux (1+ (lnfix n)) acl2::intstack bitarr)))
       (cons (cons elt bit)
             (nbalist-stobj-nbalist$c-aux (1+ (lnfix n)) acl2::intstack bitarr)))))
 
-(define nbalist-stobj-nonzero (nbalist-stobj$c)
-  :enabled t
-  (stobj-let ((acl2::intstack (nbalist-stack$c nbalist-stobj$c)))
-             (ok)
-             (not (acl2::intstack-member 0 acl2::intstack))
-             ok))
-
-
-(local (defthm pos-list-fix-when-not-member-0
-         (implies (and (acl2::u32-listp x)
-                       (not (member 0 x)))
-                  (equal (pos-list-fix x) x))
-         :hints(("Goal" :in-theory (enable acl2::u32-listp pos-list-fix)))))
-
 (define nbalist-stobj-nbalist$c (nbalist-stobj$c)
   :returns (nbalist)
-  :guard (nbalist-stobj-nonzero nbalist-stobj$c)
+  :guard (nbalist-stobj-zero-unbound nbalist-stobj$c)
   (mbe :logic (non-exec
                (nbalist-stobj-nbalist$c-logic
                 (nth *nbalist-stack$c* nbalist-stobj$c)
@@ -199,26 +385,33 @@
                         nbalist))
   ///
   (defret lookup-in-nbalist-stobj-nbalist$c
+    (implies (nbalist-stobj-zero-unbound nbalist-stobj$c)
+             (equal (hons-assoc-equal key nbalist)
+                    (and (natp key)
+                         (member key (acl2::nat-list-fix (nth *nbalist-stack$c* nbalist-stobj$c)))
+                         (cons key (bfix (nth key (nth *nbalist-bits$c* nbalist-stobj$c))))))))
+
+  (defret lookup-in-nbalist-stobj-nbalist$c-bad
     (equal (hons-assoc-equal key nbalist)
-           (and (posp key)
-                (member key (pos-list-fix (nth *nbalist-stack$c* nbalist-stobj$c)))
+           (and (natp key)
+                (member key (acl2::nat-list-fix (nth *nbalist-stack$c* nbalist-stobj$c)))
+                (not (and (equal key 0)
+                          (equal (bfix (nth key (nth *nbalist-bits$c* nbalist-stobj$c))) 0)))
                 (cons key (bfix (nth key (nth *nbalist-bits$c* nbalist-stobj$c)))))))
 
-
-
   (defret nbalistp-of-nbalist-stobj-nbalist$c
-    (implies (and (nbalist-stobj$cp nbalist-stobj$c)
-                  (nbalist-stobj-nonzero nbalist-stobj$c))
+    (implies (and (nbalist-stobj$cp nbalist-stobj$c))
              (nbalistp nbalist)))
   
   (defret len-of-<fn>
-    (implies (nbalist-stobj$cp nbalist-stobj$c)
+    (implies (and (nbalist-stobj$cp nbalist-stobj$c)
+                  (nbalist-stobj-zero-unbound nbalist-stobj$c))
              (equal (len nbalist)
                     (len (nth *nbalist-stack$c* nbalist-stobj$c))))))
 
 (defun-sk nbalist-stobj$c-size-ok (nbalist-stobj$c)
   (forall id
-          (implies (member id (pos-list-fix (nth *nbalist-stack$c* nbalist-stobj$c)))
+          (implies (member id (acl2::nat-list-fix (nth *nbalist-stack$c* nbalist-stobj$c)))
                    (< id (len (nth *nbalist-bits$c* nbalist-stobj$c)))))
   :rewrite :direct)
 
@@ -229,6 +422,7 @@
 (define nbalist-len$c (nbalist-stobj$c)
   :returns (len natp :rule-classes :type-prescription)
   :enabled t
+  :guard (nbalist-stobj-zero-unbound nbalist-stobj$c)
   (mbe :logic (len (nbalist-stobj-nbalist$c nbalist-stobj$c))
        :exec (stobj-let ((acl2::intstack (nbalist-stack$c nbalist-stobj$c)))
                         (len)
@@ -236,12 +430,12 @@
                         len)))
 
 
-(define nbalist-lookup$c ((id posp :type (unsigned-byte 32))
+(define nbalist-lookup$c ((id natp :type (unsigned-byte 32))
                           nbalist-stobj$c)
   :guard (and (non-exec (ec-call (nbalist-stobj$c-size-ok nbalist-stobj$c)))
-              (nbalist-stobj-nonzero nbalist-stobj$c))
+              (nbalist-stobj-zero-unbound nbalist-stobj$c))
   :returns (ans acl2::maybe-bitp :rule-classes :type-prescription)
-  (mbe :logic (cdr (hons-assoc-equal (pos-fix id)
+  (mbe :logic (cdr (hons-assoc-equal (nfix id)
                                      (nbalist-stobj-nbalist$c nbalist-stobj$c)))
        :exec (stobj-let ((acl2::intstack (nbalist-stack$c nbalist-stobj$c))
                          (bitarr (nbalist-bits$c nbalist-stobj$c)))
@@ -250,24 +444,23 @@
                              (get-bit id bitarr))
                         ans)))
 
-(local (defthm member-0-of-pos-list-fix
-         (not (member 0 (pos-list-fix x)))
-         :hints(("Goal" :in-theory (enable pos-list-fix)))))
 
-(define nbalist-push$c ((id posp :type (unsigned-byte 32))
+(define nbalist-push$c ((id natp :type (unsigned-byte 32))
                         (val bitp)
                         nbalist-stobj$c)
   :guard (and (non-exec (ec-call (nbalist-stobj$c-size-ok nbalist-stobj$c)))
-              (nbalist-stobj-nonzero nbalist-stobj$c)
+              (not (and (eql id 0) (eql val 0)))
+              (nbalist-stobj-zero-unbound nbalist-stobj$c)
               (not (nbalist-lookup$c id nbalist-stobj$c)))
   :returns (new-nbalist-stobj$c)
-  (mbe :logic (if (nbalist-lookup$c id nbalist-stobj$c)
+  (mbe :logic (if (or (nbalist-lookup$c id nbalist-stobj$c)
+                      (and (zp id) (eql (bfix val) 0)))
                   nbalist-stobj$c
-                (b* ((id (pos-fix id)))
+                (b* ((id (nfix id)))
                   (stobj-let ((acl2::intstack (nbalist-stack$c nbalist-stobj$c))
                               (bitarr (nbalist-bits$c nbalist-stobj$c)))
                              (acl2::intstack bitarr)
-                             (b* ((acl2::intstack (non-exec (pos-list-fix acl2::intstack)))
+                             (b* ((acl2::intstack (non-exec (acl2::nat-list-fix acl2::intstack)))
                                   (acl2::intstack (acl2::intstack-push^ id acl2::intstack))
                                   (bitarr (if (< id (bits-length bitarr))
                                               bitarr
@@ -288,11 +481,13 @@
   ///
 
   (defret nbalist-stobj-nbalist$c-of-nbalist-push$c
-    (equal (nbalist-stobj-nbalist$c new-nbalist-stobj$c)
-           (b* ((old-nbalist (nbalist-stobj-nbalist$c nbalist-stobj$c)))
-             (if (hons-assoc-equal (pos-fix id) old-nbalist)
-                 old-nbalist
-               (cons (cons (pos-fix id) (bfix val)) old-nbalist))))
+    (implies (nbalist-stobj-zero-unbound nbalist-stobj$c)
+             (equal (nbalist-stobj-nbalist$c new-nbalist-stobj$c)
+                    (b* ((old-nbalist (nbalist-stobj-nbalist$c nbalist-stobj$c)))
+                      (if (or (hons-assoc-equal (nfix id) old-nbalist)
+                              (and (zp id) (eql (bfix val) 0)))
+                          old-nbalist
+                        (cons (cons (nfix id) (bfix val)) old-nbalist)))))
     :hints(("Goal" :in-theory (enable nbalist-stobj-nbalist$c
                                       nbalist-stobj-nbalist$c-logic
                                       nbalist-lookup$c))))
@@ -307,13 +502,16 @@
                             (id (nbalist-stobj$c-size-ok-witness . ,(cdr lit)))))
                      :in-theory (disable nbalist-stobj$c-size-ok-necc))))))
 
-  (defret member-0-of-<fn>
-    (implies (not (member 0 (nth *nbalist-stack$c* nbalist-stobj$c)))
-             (not (member 0 (nth *nbalist-stack$c* new-nbalist-stobj$c))))
-    :hints(("Goal" :in-theory (enable nbalist-lookup$c)))))
+  (defret nbalist-stobj-zero-unbound-aux-of-<fn>
+    (implies (nbalist-stobj-zero-unbound-aux (nth *nbalist-stack$c* nbalist-stobj$c)
+                                             (nth *nbalist-bits$c* nbalist-stobj$c))
+             (nbalist-stobj-zero-unbound-aux (nth *nbalist-stack$c* new-nbalist-stobj$c)
+                                             (nth *nbalist-bits$c* new-nbalist-stobj$c)))
+    :hints(("Goal" :in-theory (enable nbalist-stobj-zero-unbound-aux-expand)))))
 
 (define nbalist-pop$c (nbalist-stobj$c)
-  :guard (not (equal 0 (nbalist-len$c nbalist-stobj$c)))
+  :guard (and (nbalist-stobj-zero-unbound nbalist-stobj$c)
+              (not (equal 0 (nbalist-len$c nbalist-stobj$c))))
   :returns new-nbalist-stobj$c
   (stobj-let ((acl2::intstack (nbalist-stack$c nbalist-stobj$c)))
              (acl2::intstack)
@@ -321,10 +519,12 @@
              nbalist-stobj$c)
   ///
   (defret nbalist-stobj-nbalist$c-of-nbalist-pop$c
-    (equal (nbalist-stobj-nbalist$c new-nbalist-stobj$c)
-           (cdr (nbalist-stobj-nbalist$c nbalist-stobj$c)))
+    (implies (nbalist-stobj-zero-unbound nbalist-stobj$c)
+             (equal (nbalist-stobj-nbalist$c new-nbalist-stobj$c)
+                    (cdr (nbalist-stobj-nbalist$c nbalist-stobj$c))))
     :hints(("Goal" :in-theory (enable nbalist-stobj-nbalist$c
-                                      nbalist-stobj-nbalist$c-logic))))
+                                      nbalist-stobj-nbalist$c-logic
+                                      nbalist-stobj-zero-unbound-aux-expand))))
 
   (defret nbalist-stobj$c-size-ok-of-<fn>
     (implies (nbalist-stobj$c-size-ok nbalist-stobj$c)
@@ -333,7 +533,7 @@
                  (let ((lit (assoc 'nbalist-stobj$c-size-ok clause)))
                    `(:computed-hint-replacement
                      ((and stable-under-simplificationp
-                           '(:in-theory (enable pos-list-fix))))
+                           '(:in-theory (enable acl2::nat-list-fix))))
                      :expand (,lit)
                      :use ((:instance nbalist-stobj$c-size-ok-necc
                             (id (nbalist-stobj$c-size-ok-witness . ,(cdr lit)))))
@@ -343,16 +543,23 @@
   (defret member-0-of-<fn>
     (implies (not (member 0 (nth *nbalist-stack$c* nbalist-stobj$c)))
              (not (member 0 (nth *nbalist-stack$c* new-nbalist-stobj$c))))
-    :hints(("Goal" :in-theory (enable nbalist-lookup$c)))))
+    :hints(("Goal" :in-theory (enable nbalist-lookup$c))))
+
+  (defret nbalist-stobj-zero-unbound-aux-of-<fn>
+    (implies (nbalist-stobj-zero-unbound-aux (nth *nbalist-stack$c* nbalist-stobj$c)
+                                             (nth *nbalist-bits$c* nbalist-stobj$c))
+             (nbalist-stobj-zero-unbound-aux (nth *nbalist-stack$c* new-nbalist-stobj$c)
+                                             (nth *nbalist-bits$c* new-nbalist-stobj$c)))
+    :hints(("Goal" :in-theory (enable nbalist-stobj-zero-unbound-aux-expand)))))
 
 
 (define nbalist-stobj-nthkey$c ((n natp)
                                 nbalist-stobj$c)
-  :guard (and (< n (nbalist-len$c nbalist-stobj$c))
-              (nbalist-stobj-nonzero nbalist-stobj$c))
+  :guard (and (nbalist-stobj-zero-unbound nbalist-stobj$c)
+              (< n (nbalist-len$c nbalist-stobj$c)))
   (stobj-let ((acl2::intstack (nbalist-stack$c nbalist-stobj$c)))
              (elt)
-             (lposfix (acl2::intstack-nth n acl2::intstack))
+             (lnfix (acl2::intstack-nth n acl2::intstack))
              elt))
 
 
@@ -367,22 +574,23 @@
   :enabled t
   (len (nbalist-fix nbalist)))
 
-(define nbalist-lookup ((id posp)
+(define nbalist-lookup ((id natp)
                         (nbalist nbalistp))
   :returns ans
-  (cdr (hons-get (lposfix id) (nbalist-fix nbalist))))
+  (cdr (hons-get (lnfix id) (nbalist-fix nbalist))))
 
 (local (in-theory (enable nbalist-lookup)))
 
-(define nbalist-stobj-lookup$a ((id posp :type (unsigned-byte 32))
+(define nbalist-stobj-lookup$a ((id natp :type (unsigned-byte 32))
                                 (nbalist nbalist-stobj$ap))
   :enabled t
   (nbalist-lookup id nbalist))
 
-(define nbalist-stobj-push$a ((id posp :type (unsigned-byte 32))
+(define nbalist-stobj-push$a ((id natp :type (unsigned-byte 32))
                               (val bitp)
                               (nbalist nbalist-stobj$ap))
-  :guard (not (nbalist-stobj-lookup$a id nbalist))
+  :guard (and (not (nbalist-stobj-lookup$a id nbalist))
+              (not (acl2::and** (eql id 0) (eql val 0))))
   :enabled t
   (nbalist-fix (cons (cons id val) nbalist)))
 
@@ -430,7 +638,13 @@
      :verify-guards nil
      (and (equal nbalist (nbalist-stobj-nbalist$c nbalist-stobj$c))
           (nbalist-stobj$c-size-ok nbalist-stobj$c)
-          (nbalist-stobj-nonzero nbalist-stobj$c))))
+          (nbalist-stobj-zero-unbound nbalist-stobj$c))))
+
+  (local (in-theory (disable (nbalist-stobj-zero-unbound-aux))))
+
+  (local (defthm nbalist-stobj-zero-unbound-aux-of-empty
+           (equal (nbalist-stobj-zero-unbound-aux nil nil) t)
+           :hints(("Goal" :in-theory (e/d (nbalist-stobj-zero-unbound-aux-expand))))))
 
   (local (defthm nbalist-stobj$c-size-ok-of-empty
            (nbalist-stobj$c-size-ok '(nil nil))
@@ -470,7 +684,7 @@
                                      :exec nbalist-stobj-nthkey$c))))
   
 
-(define nbalist-stobj-lookup ((id posp)
+(define nbalist-stobj-lookup ((id natp)
                               nbalist-stobj)
   :enabled t
   (mbe :logic (non-exec (nbalist-lookup id nbalist-stobj))
@@ -478,11 +692,12 @@
                  (nbalist-stobj-lookup^ id nbalist-stobj)
                (ec-call (nbalist-stobj-lookup^ id nbalist-stobj)))))
 
-(define nbalist-stobj-push ((id posp)
+(define nbalist-stobj-push ((id natp)
                             (val bitp)
                             nbalist-stobj)
   :enabled t
-  :guard (not (nbalist-stobj-lookup id nbalist-stobj))
+  :guard (and (not (nbalist-stobj-lookup id nbalist-stobj))
+              (not (acl2::and** (eql id 0) (eql val 0))))
   (mbe :logic (non-exec (nbalist-fix (cons (cons id val) nbalist-stobj)))
        :exec (if (<= id #xfffffff)
                  (nbalist-stobj-push^ id val nbalist-stobj)
