books/centaur/fgl/fgarrays.lisp
@@ -45,11 +45,6 @@
 
 (set-ignore-ok t)
 
-;; bozo add to primitives-lemmas
-(local (defthm fgl-objectlist-eval-when-atom
-         (implies (not (consp x))
-                  (equal (fgl-objectlist-eval x env) nil))
-         :hints(("Goal" :in-theory (enable fgl-objectlist-eval)))))
 
 (def-gl-primitive create-fgarray$a ()
   (b* ((next (interp-st->next-fgarray interp-st))
